# Error Analysis for Iterative Methods
## Order of Convergence
Suppose $\{p_n\}_{n=0}^{\infty}$ converges to $p$.

If $\exists \lambda \gt 0, \alpha \gt 0$ s.t:
$$
\lim_{n\to\infty} \frac{|p_{n+1}-p|}{|p_n - p|^\alpha} = \lambda
$$

then $\{p_n\}_{n=0}^{\infty}$ converges to $p$ of order $\alpha$, with asymptotic error constant $\lambda$. 

**Linearly Convergent**: - $\alpha = 1, \lambda \lt 1$
**Quadratically Convergent**: - $\alpha = 2$

Sequences with higher $\alpha$ converge *faster*.

## Fixed Point Iteration
The fixed pointer Iteration is a ***linearly convergent*** method. 

However there are conditions that allow Fixed Point Iteration to display quadratic convergence. 

For a fixed point method to converge quadratically, we need to have both $g(p) = p$, and $g'(p) = 0$.

How this will happen.

The easiest way to convert a root finding problem into a fixed point problem is to subtract a multiple of $f(x)$ from $x$.

$$
g(x) = x - \phi(x)f(x)
$$

$\phi$ will be found letter.

Notice that 
$$
g'(x) = 1 - \phi'(x)f(x) - \phi(x)f'(x)
$$

Since we know that $f(p) = 0$:
$$
g'(p) = 1 - \phi(p)f'(p)
$$

Then $g'(p) = 0$ only if $\phi(p) = 1/f'(p)$

So now we have found a way to make fixed point converge *faster*.

Notice that:
$$
p_n = g(p_{n-1}) = p_{n-1} - \phi(p_{n-1})f(p_{n-1}) = p_{n-1} - \frac{f(p_{n-1})}{f'(p_{n-1})} 
$$

This is just newtons method. 

## Multiple Roots
Recall how $f'(p) \neq 0$ for $p$ being a solution to $f(x)$. If $f'(p) = 0$ and $f(p)$ we notice that newtons/secant method gives us issues

### Definition : zero of multiplicity
A solution $p$ to $f(x) = 0$ is a zero of multiplicity $m$ of $f$ if for $x\neq p$ we can write $f(x) = (x-p)^m q(x)$, where $\lim_{x\to p}q(x) \neq 0$

If $m=1$, it is a simple zero. 

This above just says that $q(x)$  **does not**  contribute any zeros to the function at point $p$.


***Theorem***:
 $f\in C^1[a,b]$ has a simple zero and at $p\in(a, b)$ iff $f(p)=0$ but $f'(p)\neq 0$
 
 ***Theorem***:
 $f\in C^m[a,b]$ has a zero of multiplicity $m$  at $p\in(a, b)$ iff 
 $$
 0 = f(p) = f^(1)(p) = ... = f^{(m-1)}(p) \text{ but } f^{(m)}(p) \neq 0
 $$