# 4.1 Numerical Derivative Lecture 10 11 22
Recall the definition of a derivative at $x_0:$

$$
f'(x_0) = \lim_{h\to0}\frac{f(x_0+h)-f(x_0)}{h}
$$

This can be approximated trivially for small $h$ with:

$$
f'(x_0) \approx \frac{f(x_0+h)-f(x_0)}{h}
$$

## Two-Point Difference Formula & Taylor's Theorem Usage
We can use Taylor's Theorem to approximate the error:

If $f\in C^2[a, b]$, with $x_0\in[a, b]$ then:

$$
f(x) = \frac{f(x_0)}{0!} + \frac{f'(x_0)}{1!}(x-x_0) + \frac{f''(\xi(x))}{2!}(x-x_0)^2
$$

for $\xi(x)$ between $x$ and $x_0$ (what the approximation is centered around)

Using $f$ centered at $x=x_0$ lets look at $f(x_0 + h):$ 

$$
\begin{align}
f(x_0+h) &= f(x_0) + f'(x_0)h + \frac{h^2}{2}f''(\xi(x))
\\
\\
f'(x_0) &= \frac{f(x_0 + h)-f(x_0)}{h}-\underbrace{\frac{h}{2}f''(\xi(x))}_{\text{error term}}
\end{align}
$$

The bottom formula is known as the ***Two-Point Difference Formula*** for $h\gt0$ . Notice the approximation is *first-order* since the degree on $h$ is 1.

### Example
Find approximations and their errors for 

$$
\begin{align}
f&=\ln(x)\\
x_0&=1.8\\
h&\in\{.1, .05, .01\}
\end{align}
$$

$$
\begin{align}
f'(1.8) &= \frac{f(1.8 + .1)-f(1.8)}{.1} = \boxed{0.5406722}
\end{align}
$$

***Error Term***:

The error is given by $\frac{h}{2}f''(\xi) = \frac{h}{2\xi(x)^2}$

Since $\xi(x)$ is between $x_0$ and $x_0+h$ , the error term is clearly maximized at $x_0=1.8$ since adding any more $h$ will make the fraction smaller. 

Thus the error given at $h=.1$ is $\frac{.1}{2(1.8)^2} = 0.015432$

Similarly:

| $h$    | $f'(x_0)$     | *Maximized* Two Point Difference Error |
| ------ | ------------- | -------------------------- |
| $0.05$ | $0.547979483$ | $0.007716$                 |
| $0.01$ | $0.554018037$ | $0.001543$                 | 

## $n+1$ Point Formula
Suppose $S=\{x_k\}_{k=0}^{n}$ is a set of unique $n+1$ points on some interval $I$ where $f\in C^{n+1}(I)$

Then via interpolation:

$$
f(x) = \biggr[\sum_{k=0}^n f(x_k)L_k(x)\biggr] + \underbrace{\frac{(x-x_0)\times\dotso\times(x-x_n)}{(n+1)!}f^{(n+1)(\xi(x))}}_{\text{error term}}
$$

for some $\xi(x)\in I$

To approximate a derivative in $S$ we can see that 

$$
\begin{align}
f'(x) = \sum_{k=0}^n {f(x_k)}L_k'(x) + D_x\biggr[\frac{(x-x_0)\times\dotso\times(x-x_n)}{(n+1)!}f^{(n+1)(\xi(x))}\biggr]
\end{align}
$$

It is too hard to find the truncation error here unless one of the numbers here is in $S$, call it $x_j$ .

$$
\begin{align}
f'(x_j) &= \sum_{k=0}^n {f(x_k)}L_k'(x_j) + D_x\biggr[\frac{(x-x_0)\times\dotso\times(x-x_n)}{(n+1)!}f^{(n+1)(\xi(x))}\biggr] 
\\ \\
&\text{Product rule makes one of the terms go away}
\\ \\
&= \sum_{k=0}^n {f(x_k)}L_k'(x_j) + \frac{f^{(n+1)}(\xi(x_j))}{(n+1)!}\prod_{k=0,k\neq j}^n(x_j-x_k)
\end{align}
$$

> **Important**: The error term is **only** added once. It is not added per each term of the sum. 

## Three Point Formula
Consider three points: $\{x_0, x_1, x_2\}$

| $k$ | $L_k(x)$                                    | $L'_k(x)$                               |
| --- | ------------------------------------------- | --------------------------------------- |
| 0   | $\frac{(x-x_1)(x-x_2)}{(x_0-x_1)(x_0-x_2)}$ | $\frac{2x-x_1-x_2}{(x_0-x_1)(x_0-x_2)}$ |
| 1   | $\frac{(x-x_0)(x-x_2)}{(x_1-x_0)(x_1-x_2)}$ | $\frac{2x-x_0-x_2}{(x_1-x_0)(x_1-x_2)}$ |
| 2   | $\frac{(x-x_0)(x-x_1)}{(x_2-x_0)(x_2-x_1)}$ | $\frac{2x-x_0-x_1}{(x_2-x_0)(x_2-x_1)}$ |

Using the $n+1$ point formula:

$$
\begin{align}
f'(x_j) &= f(x_0)\biggr[\frac{2x-x_1-x_2}{(x_0-x_1)(x_0-x_2)}\biggr] + f(x_1)\biggr[\frac{2x-x_0-x_2}{(x_1-x_0)(x_1-x_2)}\biggr] \\ \\
&+ f(x_2)\biggr[\frac{2x-x_0-x_1}{(x_2-x_0)(x_2-x_1)}\biggr] + \frac{1}{6}f^{(3)}(\xi(x_j))\prod_{k=0,k\neq j}^2 (x_j-x_k)
\end{align}
$$

***Note:*** This formula is *only* valid for $j=0, 1, 2$

### Equidistant Points
Consider this point set where $h\neq0:$

$$
\{x_0, x_1 = x_0 + h, x_2 = x_0 + 2h\}
$$

Plugging this information into the formula above we attain:

$$
\begin{align}
f'(x_0) = f'(x_2) &= \frac{1}{h}\biggr[-\frac{3}{2}f(x_0)+2f(x_1)-\frac{1}{2}f(x_2)\biggr] + \frac{h^2}{3}f^{(3)}(\xi(x_0))
\\ \\
f'(x_1) &= \frac{1}{h}\biggr[-\frac{1}{2}f(x_0)+\frac{1}{2}f(x_2)\biggr] - \frac{h^2}{6}f^{(3)}(\xi(x_0))
\end{align}
$$

### Three-Point Endpoint Formula

$$
f'(x_0) = f'(x_0+2h) = \frac{1}{2h}\biggr[{-3}f(x_0)+4f(x_0+h)-f(x_0+2h)\biggr] + \frac{h^2}{3}f^{(3)}(\xi(x_0))
$$

### Three-Point Midpoint Formula

$$
\begin{align}
f'(x_1) = f'(x_0 + h) &= \frac{1}{2h}\biggr[-f(x_0)+f(x_0+2h)\biggr] - \frac{h^2}{6}f^{(3)}(\xi(x_0)) 
\\ \\
&\text{variable substitution of } x_0 = x_0 + h
\\ \\
f'(x_0) &= \frac{1}{2h}\biggr[-f(x_0-h)+f(x_0+h)\biggr] - \frac{h^2}{6}f^{(3)}(\xi(x_0)) 
\end{align}
$$

Notice that Three-Point Midpoint Formula requires **less** function evaluations **and** has better accuracy. 