# 4.2 Numerical Integration Lecture 10 13 22
This chapter makes the following approximation:

$$
\int_b^a f(x) \mathop{dx} = \sum_{i=0}^n a_i f(x)
$$

## Approximating $f(x)$

Consider $\{x_i\}_{i=0}^n$

We can approximate $f(x)$ given the nodes:

$$
\begin{align}
\int_b^a f(x)\mathop{dx} &= \int_b^a\sum_{i=0}^n f(x_i)L_i(x) \mathop{dx} + \int_b^a \frac{f^{n+1}(\xi(x))}{(n+1)!}\prod_{i=0}^n(x-x_i) \mathop{dx} \\ \\
&= \sum_{i=0}^n f(x_i) \underbrace{\int_b^a L_i(x) \mathop{dx}}_{a_i} + \int_b^a \frac{f^{n+1}(\xi(x))}{(n+1)!}\prod_{i=0}^n(x-x_i) \mathop{dx}\\\\ 
&= \sum_{i=0}^n a_i\cdot f(x_i) + \frac{1}{(n+1)!}\int_b^a {f^{n+1}(\xi(x))}\prod_{i=0}^n(x-x_i) \mathop{dx}\\\\ 
\end{align}
$$

## Special Cases
- Trapezoidal Rule
	- Derived from the a degree 1 Lagrange Polynomial with equally spaced nodes
- Simpson's Rule
	- Same as Trapezoidal Rule but with degree 2 Lagrange polynomials. 

## Trapezoidal Rule
Consider two nodes: $a=x_0$ and $b=x_1$ and let $h=b-a$

We can define $P_1(x)$ which will be part of the first sum term. 

$$
\begin{align}
P_1(x) &= \frac{x-x_1}{x_0 - x_1}f(x_0) + \frac{x-x_0}{x_1 - x_0}f(x_1) \\ \\
\int_{x_0}^{x_1}P_1(x) \mathop{dx} &= \int_{x_0}^{x_1} \frac{f(x_0)}{x_0-x_1}(x-x_1) \mathop{dx} + \int_{x_0}^{x_1} \frac{f(x_1)}{x_1-x_0}(x-x_0) \mathop{dx} \\ \\
&= \frac{f(x_0)(x-x_1)^2}{2(x_0-x_1)} + \frac{f(x_1)(x-x_0)^2}{2(x_1-x_0)} \biggr|_{x=x_0}^{x=x_1} \\ \\
&= \biggr(0+\frac{f(x_1)(x_1-x_0)}{2}\biggr) - \biggr(\frac{f(x_0)(x_0-x_1)}{2}+0\biggr) \\ \\
&= \frac{1}{2}(x_1-x_0)[f(x_0)+f(x_1)] \\ \\
&\implies \frac{1}{2}h(f(a)+f(b))
\end{align}
$$

We can generally use this formula for each term taking two points of the interval at a time. 