# Recap of Elim and Backsub
For the code below a look from $1:n$ will take on all values of the numbers stated. This means $1:3 = [1, 2, 3]$

## Code
### Elim
```python
# this will zero out
# each entry below a diagional (upper matrix)

for i = 1:n-1 # for each col
	for j = i+1:n # for each row
		m_ji = a_ji/a_ii
		for k = i + 1: n + 1 # move row wise
			A_jk = A_jk - (m_ji*A_jk)
```

### Backsub
```python
x_n = b_n / a_nn #b_n is just A(row=n, col=n+1) for A an aug mat

for i = n-1:1
	x_i = b_n
	for j = i+1:n 
		x_i -= a_ij * x_j
		
	x_i /= a_ii
```

## Complexity
**Summation Formulas**:

$$
\begin{align}
\sum_{j=1}^m j   &= \frac{m(m+1)}{2} \\
\sum_{j=1}^m j^2 &= \frac{m(m+1)(2m+1)}{6}
\end{align}
$$

### Elim Code
In the $k$ loop there are $(n+1) - (i+1) + 1$ mults with $(n+1) - (i+1) + 1$ subtractions. 

In the $j$ loop there is $n - (i + 1) + 1 = n - i$ divs. 

Since loop $k$ is inside $j$ the results are multiplied:

$$
\begin{align}
\text{mult/div} &= (n - i)(n-i+1)+\underbrace{(n - i)}_{\text{calc } m_{ji}} = (n - i)(n-i+1)\\ 
\text{add/sub} &= (n - i)(n-i+1)\\ 
\end{align}
$$

The outer $i$ is what controls $j, k$. Thus the total number of add/sub operations is based on:

$$
\sum_{i=1}^{n-1} (n-i)(n-i+1)
$$

$$
\begin{align}
\sum_{i=1}^{n-1} (n-i)(n-i+1) &= \sum_{i=1}^{n-1} \underbrace{n^2-2ni+i^2}_{(n-i)^2} + n - i \\ \\
&= \sum_{i=1}^{n-1} (n-i)^2 + \sum_{i=1}^{n-1} (n-i) \\ \\
&= \sum_{i=1}^{n-1} (i)^2 + \sum_{i=1}^{n-1} (i) \\ \\
&= \dotso (\text{ algebra }) \\
&= \frac{n^3 - n}{3}
\end{align}
$$

The mult/div count can be obtained the same way:

$$
\sum_{i=1}^{n-1} (n-i)(n-i+2) = \frac{2n^3+3n^2-5n}{6}
$$

The total number of operations is the sum of add/subs and mults/divs:

$$
\sum_{i=1}^{n-1} (n-i)(n-i+2) + \sum_{i=1}^{n-1} (n-i)(n-i+1) = \frac{4n^3+3n^2-7n}{6} \in O\left(\frac{2}{3}n^3\right)
$$

### Backsub Code

In short the total number of operations are $n^2$

# Matrix Factorization

We want to find $\bar{x}$ s.t $A\bar{x}=\bar{b}$

We can attempt to find $L, U$ s,t $LU = A$

$$
\begin{align}
&A = LU \implies LU\bar{x}=\bar{b} \\
\text{Let } &\bar{y} = U\bar{x} \implies L\bar{y} = \bar{b}
\end{align}
$$

Since L and U are lower and upper matrices, forward substitution and backward substitution can reduce compute time. 

**What is forward substitution**

Realize that 

$$
L = 
\begin{bmatrix}
* & 0 & \dotso & 0 \\
\vdots & \ddots & 0 & 0\\
* & * & \dotso & *
\end{bmatrix}
$$

We can start with $L_{11}$ and work our way down to find all the $x_i$ .

### How to find U - $2\times2$

$$
A = 
\begin{bmatrix}
1 & 1 \\
3 & -4 \\
\end{bmatrix}
\stackrel{E_2-3E_1}{\to}
\underbrace{
\begin{bmatrix}
1 & 1 \\
0 & -7 \\
\end{bmatrix}
}_U
$$

Notice we subtracted $3E_1$ from $E_2$ To undo this we need to add $3E_1$ to get back to $A$. 

Therefore: 

$$
L = \begin{bmatrix}
1 & 0 \\
3 & 1 \\
\end{bmatrix}
$$

To get back to row one we keep it the same (row 1 was unchanged)

To get back to row two we need to add $3E_1$ to the current row. 

Notice the 2nd row of $U$ . From $L$ we need $3E_1 + E_2$ from the original matrix to get back to A. 