# 7.3 Iterative Methods Lecture 11 15 22
Start with a guess $\bar{x}^{(0)}$ and generate a sequence of vectors $\{\bar{x}\}_{k=0}^{\infty}$ that converges to $\bar{x}$

## Defining Vector Convergence
$\{\bar{x}\}_{k=0}^{\infty}$ converge to $\bar{x}$ WRT to a specific norm $\|\cdot\|$ if given a $\epsilon\gt0,\ \exists N(\epsilon)\in\mathbb{N}$ s.t

$$
\|\bar{x}^{(k)}-\bar{x}\| \lt \epsilon \,\,\, \forall k\geq N(\epsilon)
$$

***Theorem***:

$\{\bar{x}\}_{k=0}^{\infty}$ converges to $\bar{x} \in \mathbb{R}^n$ WRT $\ell_\infty \iff \lim_{k\to\infty} x_i^{(k)}=x_i \ \forall i=1,\dotso,n$

### Proof
####  $p\to q$
Given that the vector sequence converges, $\forall \epsilon\gt0,\ \exists N(\epsilon)\in\mathbb{N}$ s.t $\|\bar{x}^{(k)}-\bar{x}\|_\infty \lt \epsilon \ \forall k\geq N(\epsilon)$

However $\|\bar{x}^{(k)}-\bar{x}\|_\infty = \max_{i=1,\dotso, n}|x_i^{(k)}-x_i|\lt \epsilon$

Since the largest difference between components is less than $\epsilon$, by definition of the limit:

$$
\lim_{k\to\infty} x_i^{(k)} = x_i
$$

#### $q\to p$
Given an $\epsilon\gt0$ , $\exists N_i(\epsilon)\in\mathbb{N}$ such that $|x_i^{(k)} - x_i|\lt\epsilon$ for all $k\gt N_i(\epsilon)$

> The above is the definition of the limit which is given. 

Define a $N(\epsilon)=\max_{i=1, \dotso, n}\biggr(N_i(\epsilon)\biggr)$

Then $\forall k\gt N(\epsilon),\ |x_{i}^{(k)}-x_i|\lt\epsilon$ for any $i$ .

If all components converge, the vector converges:

$$
\{\bar{x}^{(k)}\}_{k=0}^{\infty} \to \bar{x}
$$

## Jacobi Iterative Method
Idea: solve the $i\text{-th}$ equation for $x_i$ (assert $x_{ii}\neq0$)

Here is a general form for the $i\text{-th}$ equation.

$$
a_{i1}x_1 + \dotso + a_{ii}x_i + \dotso + a_{in}x_n = b_i
$$

We can find $x_i$ with the formula below.

$$
x_i = \frac{1}{a_{ii}}\biggr(
b_i -
\sum_{j=1,\ j\neq i}^n a_{ij}x_j
\biggr)
\text{ for }
i = 1,\dotso, n
$$

This is where the initial guess comes in:

For $k\geq1$ you obtain $\bar{x}^{(k)}$ from $\bar{x}^{(k-1)}$

$$
x_i^{(k)} = \frac{1}{a_{ii}}\biggr(
b_i -
\sum_{j=1,\ j\neq i}^n a_{ij}x_j^{(k-1)}
\biggr)
$$

### Example

$$
[ \ A \ | \ \bar{b} \ ] =
\begin{bmatrix}
3 & 1 & 5 \\
1 & 2 & 5 \\
\end{bmatrix}
$$

Our initial guess can be $\bar{x}^{(0)}=[0\ 0]^T$

Then we can define the relations.

$$
\begin{align}
x_1^{(k)} &= \frac{5-x_2^{(k-1)}}{3} \\
x_2^{(k)} &= \frac{5-x_1^{(k-1)}}{2}
\end{align}
$$

Here are the results for $k=1, 2, 3$

$$
\begin{align}
k = 1 &\to [5/3\ 5/2]^T \\
k = 2 &\to [5/6\ 5/3]^T \\
k = 3 &\to [10/9\ 25/12]^T
\end{align}
$$

## Jacobi Iterative Method - Matrix Formation
Lets first define relevant matrices:

$$
\begin{align}
D &= 
\begin{bmatrix}
a_{11} & 0 & \cdots & 0 \\
0 & a_{22} & \cdots & 0 \\
\vdots & \vdots &\ddots & \vdots\\
0 & 0 & \cdots & a_{nn} \\
\end{bmatrix}
\\ \\
L &= 
\begin{bmatrix}
0 & 0 & \cdots & 0  &  0 \\
-a_{21} & 0 & \cdots & 0 & 0 \\
-a_{31} & -a_{32} & \cdots & 0 & 0 \\
\vdots & \vdots &\ddots & \vdots & \vdots\\
-a_{n1} & -a_{n2} & \cdots & -a_{n, n-1} & 0 \\
\end{bmatrix}
\\ \\
U &= 
\begin{bmatrix}
0 & -a_{12} & -a_{13} & \dotso & -a_{1n} \\
0 & 0 & -a_{23} & \dotso & -a_{2n} \\
\vdots & \vdots & \ddots & \vdots & \vdots \\
0 & 0 & \dots & 0 & -a_{n-1, n} \\
0 & 0 & \dots & 0 & 0 \\
\end{bmatrix}
\end{align}
$$

See that $A = D - L -U$ which implies that $(D-L-U)\bar{x} = \bar{b}$

$$
\begin{align}
D\bar{x} &= (L+U)\bar{x} + \bar{b} \\
\bar{x} &= D^{-1}(L+U)\bar{x} + D^{-1}\bar{b} \\
\implies \bar{x}^{(k)} &= \underbrace{D^{-1}(L+U)}_{T_j}\bar{x}^{(k-1)} + \underbrace{D^{-1}\bar{b}}_{C_j}
\end{align}
$$

For this algorithm to work we may reorder $E_i$ to ensure there is no $i$ such that $a_{ii} = 0$ and for speed we should ensure $|a_{ii}|$ is large. 