# 1.3 Zero Convergence
> From Homework 1, Q7d

Find the rate of convergence of 

$$
\lim_{h\to0}\frac{1-e^h}{h} = -1
$$

$$
\begin{align}
e^h &= P_1(x) + R_1(x) \\
&= e^0 + e^0h + e^{[\xi(h)]}\frac{h^2}{2},\ \xi(h) \text{ beteween } 0 \text{ and } h
\end{align}
$$

Back to the expression:

$$
\frac{1-e^h}{h} = \frac{1-\biggr[e^0 + e^0h + e^{[\xi(h)]}\frac{h^2}{2}\biggr]}{h} = -1 - e^{[\xi(h)]}\frac{h}{2}
$$

Then:

$$
\biggr| \frac{1-e^h}{h} - (-1) \biggr| =\ \biggr| -1 - e^{[\xi(h)]}\frac{h}{2} - (-1) \biggr| =\ \biggr| -e^{[\xi(h)]} \biggr|\biggr| \frac{h}{2} \biggr| \leq e^{\max(0, h)} \biggr| \frac{h}{2} \biggr| = \frac{e^{\max(0, h)}}{2} |h|
$$

Since $\exists k \in \mathbb{R}$ s.t $\biggr| \frac{1-e^h}{h} - (-1) \biggr| \leq k|h|$, 

$$
\boxed{\frac{1-e^h}{h} = -1 + O(h)}
$$